Make more generic, refactor code a bit more.

CrIdentifiers.v
@@ -13,26 +13,3 @@ Inductive ModuleName : Type := ModuleNameCtr (name : string).
 Inductive FunctionName : Type := FunctionNameCtr (name : string).
 Inductive ConnectionName : Type := ConnectionNameCtr (name : string).
 Inductive CtrlPlaneConfigName : Type := CtrlPlaneConfigNameCtr (name : string).
-
-(* Current values for each of these identifiers as a map *)
-Definition HeaderMap (T : Type) := Header -> T.
-Definition StateVarMap (T : Type) := StateVar -> T.
-Definition CtrlPlaneConfigNameMap (T : Type) := CtrlPlaneConfigName -> T.
-
-Definition update_hdr_map (s: HeaderMap uint8) (x: Header) (v: uint8) : (HeaderMap uint8) :=
-  fun y => match x, y with
-            | HeaderCtr x_name, HeaderCtr y_name => if string_dec x_name y_name then v else s y
-           end.
-
-Definition update_state_map (s: StateVarMap uint8) (x: StateVar) (v: uint8) : (StateVarMap uint8) :=
-  fun y => match x, y with
-            | StateVarCtr x_name, StateVarCtr y_name => if string_dec x_name y_name then v else s y
-           end.
-
-(* The ProgramState is a record containing three maps:,
-   one each for mapping headers/statevars/ctrlplaneconfigs to their current values *)
-Record ProgramState := {
-  ctrl_plane_map : CtrlPlaneConfigNameMap uint8;
-  header_map : HeaderMap uint8;
-  state_var_map : StateVarMap uint8
-}.
