CrProgramState.v
@@ -1,0 +1,25 @@
+From MyProject Require Export CrIdentifiers.
+Require Import Strings.String.
+
+(* Current values for each of these identifiers as a map *)
+Definition HeaderMap (T : Type) := Header -> T.
+Definition StateVarMap (T : Type) := StateVar -> T.
+Definition CtrlPlaneConfigNameMap (T : Type) := CtrlPlaneConfigName -> T.
+
+Definition update_hdr_map {T : Type} (s: HeaderMap T) (x: Header) (v: T) : (HeaderMap T) :=
+  fun y => match x, y with
+            | HeaderCtr x_name, HeaderCtr y_name => if string_dec x_name y_name then v else s y
+           end.
+
+Definition update_state_map {T : Type} (s: StateVarMap T) (x: StateVar) (v: T) : (StateVarMap T) :=
+  fun y => match x, y with
+            | StateVarCtr x_name, StateVarCtr y_name => if string_dec x_name y_name then v else s y
+           end.
+
+(* The ProgramState is a record containing three maps:,
+   one each for mapping headers/statevars/ctrlplaneconfigs to their current values *)
+Record ProgramState (T : Type) := {
+  ctrl_plane_map : CtrlPlaneConfigNameMap T;
+  header_map : HeaderMap T;
+  state_var_map : StateVarMap T
+}.
