CrTransformer.v
@@ -6,6 +6,7 @@ Require Import ZArith.
 Import ListNotations.
 Require Import Strings.String.
 From MyProject Require Export CrIdentifiers.
+From MyProject Require Export CrProgramState.
 
 (* A transformer is either a sequential or a parallel transformer *)
 Inductive TransformerType : Type := 
@@ -19,12 +20,12 @@ Inductive FunctionArgument :=
   | StatefulArg (s : StateVar).
 
 (* lookup a function's argument *)
-Definition function_argument_to_uint8 (arg : FunctionArgument) (valuation : ProgramState) : uint8 :=
+Definition function_argument_to_uint8 (arg : FunctionArgument) (valuation : ProgramState uint8) : uint8 :=
   match arg with
-  | CtrlPlaneArg c => valuation.(ctrl_plane_map) c
-  | HeaderArg h    => valuation.(header_map) h
+  | CtrlPlaneArg c => ctrl_plane_map uint8 valuation c
+  | HeaderArg h    => header_map uint8 valuation h
   | ConstantArg n  => n
-  | StatefulArg s  => valuation.(state_var_map) s
+  | StatefulArg s  => state_var_map uint8 valuation s
   end.
 
 (* A BinaryOp takes two uint8 arguments and returns another uint8 *)
